\smalltitle{سوال 4}
\begin{gather*}
    \mathcal{L} (x_1, \cdots, x_n; \lambda) \stackrel{i.i.d.}{=} \prod_{i=1}^n f(x_i; \lambda)
    = \prod_{i=1}^n \frac{\lambda^k x_i^{k-1} e^{-\lambda x}}{(k-1)!} = \frac{\lambda^{nk}}{(k-1)!^n} e^{-\lambda (\sum_{i=1}^n x_i)} \prod_{i=1}^n x_i^{k-1}\\
    \stackrel{\ln}{=} nk \ln \lambda - n\ln((k-1)!) -\lambda (\sum_{i=1}^n x_i) + (k-1) \sum_{i=1}^n \ln(x_i)\\
    \stackrel{\frac{d}{d \lambda}}{=} \frac{nk}{\lambda} = \sum_{i=1}^n x_i
    \implies \lambda = \frac{k}{\overline{x}}
\end{gather*}